WIP: moved enc to own typeclass TODO: port extraction?

theories/L/Datatypes/LDepPair.v
@@ -6,14 +6,15 @@ Section sigT.
   Variable A : Type.
   Context `{reg_A : registered A}.
   Variable P : A -> Type.
-  Context `{reg_P : forall x, registered (P x)}.
+  Context `{enc_P : forall x, encodable (P x)}.
+  Context {reg_P : forall x, registered (P x)}.
 
-  Definition sigT_enc : encodable (sigT P) :=
+  Instance sigT_enc : encodable (sigT P) :=
     fun '@existT _ _ x y => lam (0 (enc x) (enc y)).
   
   Global Instance registered_sigT : registered (sigT P).
   Proof.
-    exists sigT_enc.
+    split.
     -intros []. cbn. Lproc.
     -intros [] [] H. inv H. eapply inj_enc in H1. subst x. apply inj_enc in H2. subst p. easy.
   Defined.
